STLC/Readme.txt
@@ -1,0 +1,5 @@
+Definitions.v contains the basic definition of our language.
+Initial.v contains the initial CPS conversion function.
+PatternMatch.v contains the CPS conversion function which deals with nested pattern match.
+Argument.v contains the CPS conversion function which deals with the case where recursive calls appear in the arguments of another recursive call.
+Proof.v contains an informal proof of the final CPS conversion function.
